<?xml version="1.0" encoding="utf-8"?>
<rdf:RDF xmlns:dcat="http://www.w3.org/ns/dcat#" xmlns:dct="http://purl.org/dc/terms/" xmlns:gsp="http://www.opengis.net/ont/geosparql#" xmlns:owl="http://www.w3.org/2002/07/owl#" xmlns:rdf="http://www.w3.org/1999/02/22-rdf-syntax-ns#" xmlns:rdfs="http://www.w3.org/2000/01/rdf-schema#" xmlns:skos="http://www.w3.org/2004/02/skos/core#" xmlns:xkos="http://rdf-vocabulary.ddialliance.org/xkos#" xmlns:xsd="http://www.w3.org/2001/XMLSchema#" xmlns:wdrs="http://www.w3.org/2007/05/powder-s#" xmlns:ft="http://publications.europa.eu/resource/authority/file-type/" xmlns:mt="https://www.iana.org/assignments/media-types/">
  <rdf:Description rdf:about="https://ipsoeu.github.io/cos-taxonomy/life-event/2019">
    <rdf:type rdf:resource="http://www.w3.org/ns/dcat#Dataset"/>
    <rdf:type rdf:resource="http://www.w3.org/2004/02/skos/core#ConceptScheme"/>
    <dct:identifier>life-event-2019</dct:identifier>
    <owl:versionInfo>2019</owl:versionInfo>
    <dct:isVersionOf rdf:resource="https://ipsoeu.github.io/cos-taxonomy/life-event"/>
    <dct:title xml:lang="en">Life events</dct:title>
    <dct:description xml:lang="en">Life events</dct:description>
    <dct:issued rdf:datatype="http://www.w3.org/2001/XMLSchema#date">2019-09-04</dct:issued>
    <dct:valid rdf:datatype="http://www.w3.org/2001/XMLSchema#date">2019-09-04</dct:valid>
    <wdrs:validfrom rdf:datatype="http://www.w3.org/2001/XMLSchema#date">2019-09-04</wdrs:validfrom>
    <wdrs:validuntil rdf:datatype="http://www.w3.org/2001/XMLSchema#date">2019-09-04</wdrs:validuntil>
    <dcat:landingPage rdf:resource="https://ipsoeu.github.io/cos-taxonomy/life-event/2019"/>
    <rdfs:isDefinedBy rdf:resource="https://joinup.ec.europa.eu/sites/default/files/news/2019-09/ISA2_European%20taxonomy%20for%20public%20services.pdf"/>
    <skos:hasTopConcept rdf:resource="https://ipsoeu.github.io/cos-taxonomy/life-event/2019/LE01"/>
    <skos:hasTopConcept rdf:resource="https://ipsoeu.github.io/cos-taxonomy/life-event/2019/LE02"/>
    <skos:hasTopConcept rdf:resource="https://ipsoeu.github.io/cos-taxonomy/life-event/2019/LE03"/>
    <skos:hasTopConcept rdf:resource="https://ipsoeu.github.io/cos-taxonomy/life-event/2019/LE04"/>
    <skos:hasTopConcept rdf:resource="https://ipsoeu.github.io/cos-taxonomy/life-event/2019/LE05"/>
    <skos:hasTopConcept rdf:resource="https://ipsoeu.github.io/cos-taxonomy/life-event/2019/LE06"/>
    <skos:hasTopConcept rdf:resource="https://ipsoeu.github.io/cos-taxonomy/life-event/2019/LE07"/>
    <skos:hasTopConcept rdf:resource="https://ipsoeu.github.io/cos-taxonomy/life-event/2019/LE08"/>
    <skos:hasTopConcept rdf:resource="https://ipsoeu.github.io/cos-taxonomy/life-event/2019/LE09"/>
    <skos:hasTopConcept rdf:resource="https://ipsoeu.github.io/cos-taxonomy/life-event/2019/LE10"/>
    <skos:hasTopConcept rdf:resource="https://ipsoeu.github.io/cos-taxonomy/life-event/2019/LE11"/>
    <skos:hasTopConcept rdf:resource="https://ipsoeu.github.io/cos-taxonomy/life-event/2019/LE12"/>
    <skos:hasTopConcept rdf:resource="https://ipsoeu.github.io/cos-taxonomy/life-event/2019/LE13"/>
  </rdf:Description>
  <rdf:Description rdf:about="https://ipsoeu.github.io/cos-taxonomy/life-event/2019/LE01">
    <rdf:type rdf:resource="http://www.w3.org/2004/02/skos/core#Concept"/>
    <dct:identifier>LE01</dct:identifier>
    <skos:notation>LE01</skos:notation>
    <skos:prefLabel xml:lang="en">Having a child</skos:prefLabel>
    <skos:definition xml:lang="en">This life event groups public services related to becoming a caretaker for a child, for instance in case of giving birth, adopting, receiving a foster child…</skos:definition>
    <skos:inScheme rdf:resource="https://ipsoeu.github.io/cos-taxonomy/life-event/2019"/>
    <skos:topConceptOf rdf:resource="https://ipsoeu.github.io/cos-taxonomy/life-event/2019"/>
  </rdf:Description>
  <rdf:Description rdf:about="https://ipsoeu.github.io/cos-taxonomy/life-event/2019/LE02">
    <rdf:type rdf:resource="http://www.w3.org/2004/02/skos/core#Concept"/>
    <dct:identifier>LE02</dct:identifier>
    <skos:notation>LE02</skos:notation>
    <skos:prefLabel xml:lang="en">Becoming a (social) caretaker</skos:prefLabel>
    <skos:definition xml:lang="en">This life event groups public services related to the situation where you need to take care of another person (other than when you get a child), for instance for an elder, a disabled person…</skos:definition>
    <skos:inScheme rdf:resource="https://ipsoeu.github.io/cos-taxonomy/life-event/2019"/>
    <skos:topConceptOf rdf:resource="https://ipsoeu.github.io/cos-taxonomy/life-event/2019"/>
  </rdf:Description>
  <rdf:Description rdf:about="https://ipsoeu.github.io/cos-taxonomy/life-event/2019/LE03">
    <rdf:type rdf:resource="http://www.w3.org/2004/02/skos/core#Concept"/>
    <dct:identifier>LE03</dct:identifier>
    <skos:notation>LE03</skos:notation>
    <skos:prefLabel xml:lang="en">Starting education</skos:prefLabel>
    <skos:definition xml:lang="en">This life event groups any public service related to education, for example pre-school education, elementary school, higher education and university…</skos:definition>
    <skos:inScheme rdf:resource="https://ipsoeu.github.io/cos-taxonomy/life-event/2019"/>
    <skos:topConceptOf rdf:resource="https://ipsoeu.github.io/cos-taxonomy/life-event/2019"/>
  </rdf:Description>
  <rdf:Description rdf:about="https://ipsoeu.github.io/cos-taxonomy/life-event/2019/LE04">
    <rdf:type rdf:resource="http://www.w3.org/2004/02/skos/core#Concept"/>
    <dct:identifier>LE04</dct:identifier>
    <skos:notation>LE04</skos:notation>
    <skos:prefLabel xml:lang="en">Looking for a new job</skos:prefLabel>
    <skos:definition xml:lang="en">This life event groups public services for when someone looks for a new job or starts a new job.</skos:definition>
    <skos:inScheme rdf:resource="https://ipsoeu.github.io/cos-taxonomy/life-event/2019"/>
    <skos:topConceptOf rdf:resource="https://ipsoeu.github.io/cos-taxonomy/life-event/2019"/>
  </rdf:Description>
  <rdf:Description rdf:about="https://ipsoeu.github.io/cos-taxonomy/life-event/2019/LE05">
    <rdf:type rdf:resource="http://www.w3.org/2004/02/skos/core#Concept"/>
    <dct:identifier>LE05</dct:identifier>
    <skos:notation>LE05</skos:notation>
    <skos:prefLabel xml:lang="en">Losing/quitting a job</skos:prefLabel>
    <skos:definition xml:lang="en">This life event groups public services related to the situation when someone leaves or quits a particular jobs on his own, or when someone loses his job, for instance getting fired, collective dismissal, in case of failure of the company…</skos:definition>
    <skos:inScheme rdf:resource="https://ipsoeu.github.io/cos-taxonomy/life-event/2019"/>
    <skos:topConceptOf rdf:resource="https://ipsoeu.github.io/cos-taxonomy/life-event/2019"/>
  </rdf:Description>
  <rdf:Description rdf:about="https://ipsoeu.github.io/cos-taxonomy/life-event/2019/LE06">
    <rdf:type rdf:resource="http://www.w3.org/2004/02/skos/core#Concept"/>
    <dct:identifier>LE06</dct:identifier>
    <skos:notation>LE06</skos:notation>
    <skos:prefLabel xml:lang="en">Looking for a place to live</skos:prefLabel>
    <skos:definition xml:lang="en">This life event groups public services related to a person’s place of living, for instance, changing residence, buying a house or a piece of land, building, renting a house or apartment…</skos:definition>
    <skos:inScheme rdf:resource="https://ipsoeu.github.io/cos-taxonomy/life-event/2019"/>
    <skos:topConceptOf rdf:resource="https://ipsoeu.github.io/cos-taxonomy/life-event/2019"/>
  </rdf:Description>
  <rdf:Description rdf:about="https://ipsoeu.github.io/cos-taxonomy/life-event/2019/LE07">
    <rdf:type rdf:resource="http://www.w3.org/2004/02/skos/core#Concept"/>
    <dct:identifier>LE07</dct:identifier>
    <skos:notation>LE07</skos:notation>
    <skos:prefLabel xml:lang="en">Changing relationship status</skos:prefLabel>
    <skos:definition xml:lang="en">This life event groups public services related to a person’s official relationship, for instance marriage, registered partnership, divorce…</skos:definition>
    <skos:inScheme rdf:resource="https://ipsoeu.github.io/cos-taxonomy/life-event/2019"/>
    <skos:topConceptOf rdf:resource="https://ipsoeu.github.io/cos-taxonomy/life-event/2019"/>
  </rdf:Description>
  <rdf:Description rdf:about="https://ipsoeu.github.io/cos-taxonomy/life-event/2019/LE08">
    <rdf:type rdf:resource="http://www.w3.org/2004/02/skos/core#Concept"/>
    <dct:identifier>LE08</dct:identifier>
    <skos:notation>LE08</skos:notation>
    <skos:prefLabel xml:lang="en">Driving a vehicle</skos:prefLabel>
    <skos:definition xml:lang="en">This life event groups public services related to driving a vehicle, for instance car, motorcycle… Some example public services are getting your driver license, following driving lessons, registering your car…</skos:definition>
    <skos:inScheme rdf:resource="https://ipsoeu.github.io/cos-taxonomy/life-event/2019"/>
    <skos:topConceptOf rdf:resource="https://ipsoeu.github.io/cos-taxonomy/life-event/2019"/>
  </rdf:Description>
  <rdf:Description rdf:about="https://ipsoeu.github.io/cos-taxonomy/life-event/2019/LE09">
    <rdf:type rdf:resource="http://www.w3.org/2004/02/skos/core#Concept"/>
    <dct:identifier>LE09</dct:identifier>
    <skos:notation>LE09</skos:notation>
    <skos:prefLabel xml:lang="en">Travelling abroad</skos:prefLabel>
    <skos:definition xml:lang="en">This life events groups public services related to what you need to do when travelling abroad, for instance getting an international passport or driving license, getting a visa, getting vaccination…</skos:definition>
    <skos:inScheme rdf:resource="https://ipsoeu.github.io/cos-taxonomy/life-event/2019"/>
    <skos:topConceptOf rdf:resource="https://ipsoeu.github.io/cos-taxonomy/life-event/2019"/>
  </rdf:Description>
  <rdf:Description rdf:about="https://ipsoeu.github.io/cos-taxonomy/life-event/2019/LE10">
    <rdf:type rdf:resource="http://www.w3.org/2004/02/skos/core#Concept"/>
    <dct:identifier>LE10</dct:identifier>
    <skos:notation>LE10</skos:notation>
    <skos:prefLabel xml:lang="en">Moving to/from the country</skos:prefLabel>
    <skos:definition xml:lang="en">This life event groups public services that relate to when someone moves from one country to another.</skos:definition>
    <skos:inScheme rdf:resource="https://ipsoeu.github.io/cos-taxonomy/life-event/2019"/>
    <skos:topConceptOf rdf:resource="https://ipsoeu.github.io/cos-taxonomy/life-event/2019"/>
  </rdf:Description>
  <rdf:Description rdf:about="https://ipsoeu.github.io/cos-taxonomy/life-event/2019/LE11">
    <rdf:type rdf:resource="http://www.w3.org/2004/02/skos/core#Concept"/>
    <dct:identifier>LE11</dct:identifier>
    <skos:notation>LE11</skos:notation>
    <skos:prefLabel xml:lang="en">Going into military service</skos:prefLabel>
    <skos:definition xml:lang="en">This life event groups public services related to taking up a mandatory military or civil service.</skos:definition>
    <skos:inScheme rdf:resource="https://ipsoeu.github.io/cos-taxonomy/life-event/2019"/>
    <skos:topConceptOf rdf:resource="https://ipsoeu.github.io/cos-taxonomy/life-event/2019"/>
  </rdf:Description>
  <rdf:Description rdf:about="https://ipsoeu.github.io/cos-taxonomy/life-event/2019/LE12">
    <rdf:type rdf:resource="http://www.w3.org/2004/02/skos/core#Concept"/>
    <dct:identifier>LE12</dct:identifier>
    <skos:notation>LE12</skos:notation>
    <skos:prefLabel xml:lang="en">Facing an emergency / health problem</skos:prefLabel>
    <skos:definition xml:lang="en">This life event groups public services related to when someone faces an emergency, for instance in the case of an accident, or a severe health problem, for instance getting disabled.</skos:definition>
    <skos:inScheme rdf:resource="https://ipsoeu.github.io/cos-taxonomy/life-event/2019"/>
    <skos:topConceptOf rdf:resource="https://ipsoeu.github.io/cos-taxonomy/life-event/2019"/>
  </rdf:Description>
  <rdf:Description rdf:about="https://ipsoeu.github.io/cos-taxonomy/life-event/2019/LE13">
    <rdf:type rdf:resource="http://www.w3.org/2004/02/skos/core#Concept"/>
    <dct:identifier>LE13</dct:identifier>
    <skos:notation>LE13</skos:notation>
    <skos:prefLabel xml:lang="en">Facing a crime</skos:prefLabel>
    <skos:definition xml:lang="en">This life event groups public services related to a crime, for instance in case related to a crime, for instance in case</skos:definition>
    <skos:inScheme rdf:resource="https://ipsoeu.github.io/cos-taxonomy/life-event/2019"/>
    <skos:topConceptOf rdf:resource="https://ipsoeu.github.io/cos-taxonomy/life-event/2019"/>
  </rdf:Description>
</rdf:RDF>
